
\chapter{Derivation of implicit backwards difference formulae}
\label{cha:deriv-impl-backw}

Starting from \cref{eq:59} and setting $\pv_k(t_{n+1}) = \ffv{t_{n+1}, \yv_{n+1}}$ we obtain
\begin{equation}
  \begin{aligned}
    \fv(t_{n+1}, \yv_{n+1}) &= \sum_{j=1}^k \yv[t_{n+1}, \ldots, t_{n+1-j}] \sum_{l=0}^{j-1} \prod_{i=0, i \neq l}^{j-1} (t_{n+1} - t_{n+1-i}).
  \end{aligned}
\end{equation}
This can be greatly simplified by noticing that the product $ \prod_{i=0, i \neq l}^{j-1} (t_{n+1} - t_{n+1-i})$ is zero whenever it contains $i=0$, \ie all terms in the sum with $l \neq 0$.
This leaves us with
\begin{equation}
  \begin{aligned}
    \fv(t_{n+1}, \yv_{n+1}) &= \sum_{j=1}^k \yv[t_{n+1}, \ldots, t_{n+1-j}] \prod_{i=0, i \neq 0}^{j-1} (t_{n+1} - t_{n+1-i}), \\
    &=  \yv[t_{n+1}, t_n] + \sum_{j=2}^k \yv[t_{n+1}, \ldots, t_{n+1-j}] \prod_{i=1}^{j-1} (t_{n+1} - t_{n+1-i}). \\
  \end{aligned}
\end{equation}

For $k=1$ we get
\begin{equation}
  \begin{aligned}
    \fv(t_{n+1}, \yv_{n+1}) &= \frac{\yv_{n+1} - \yv_n}{\dtn}, \\
    \yv_{n+1} &= \yv_n + \dtn \fv(t_{n+1}, \yv_{n+1}),
  \end{aligned}
\end{equation}
which is backward Euler as expected.

For $k=2$
\begin{equation}
  \label{eqn:bdf2-derivation}
  \begin{aligned}
    \fv(t_{n+1}, \yv_{n+1}) &= \frac{\yv_{n+1} - \yv_n}{\dtn} +  \yv[t_{n+1}, t_{n}, t_{n-1}](t_{n+1} - t_n), \\
    &= \frac{\yv_{n+1} - \yv_n}{\dtn} +  \frac{\dtn}{\dtx{n+1} + \dtn} \bigb{\frac{\yv_{n+1} - \yv_n}{\dtn} - \frac{\yv_n - \yv_{n-1}}{\dtx{n-1}}}. \\
  \end{aligned}
\end{equation}
After some algebra this becomes
\begin{equation}
  \label{eqn:bdf2-derivation-rearranged}
  \begin{aligned}
    \frac{\yv_{n+1} - \yv_n}{\dtn} = \frac{\dtn}{2\dtn + \dtx{n-1}} \frac{\yv_n - \yv_{n-1}}{\dtx{n-1}}
    + \frac{\dtn + \dtx{n-1}}{2\dtn + \dtx{n-1}} \fv(t_{n+1}, \yv_{n+1}),
  \end{aligned}
\end{equation}
which is variable step BDF2 \cite[715]{GreshoSani}.

%%% Local Variables:
%%% mode: latex
%%% TeX-master: "main"
%%% End:
